Veir/Rewriter/WellFormed/Builder/OpRegion.lean
@@ -5,8 +5,8 @@ import Veir.Rewriter.Basic
 namespace Veir
 
 set_option warn.sorry false in
-theorem Rewriter.initOpRegions_WellFormed (ctx: IRContext) (opPtr: OperationPtr) (numRegions: Nat)
+theorem Rewriter.initOpRegions_WellFormed (opPtr: OperationPtr)
     (hop : opPtr.InBounds ctx) (hctx : IRContext.WellFormed ctx) (newCtx : IRContext):
-    Rewriter.initOpRegions ctx opPtr numRegions hop = some newCtx →
+    Rewriter.initOpRegions ctx opPtr regions n hop regionInBounds (by grind) hn = some newCtx →
     newCtx.WellFormed := by
   sorry
